sf/Assignment08_04.v
@@ -1,4 +1,4 @@
-Require Export Assignment08_03.
+git diffvfRequire Export Assignment08_03.
 
 (* problem #04: 10 points *)
 
@@ -13,7 +13,23 @@ Theorem no_whiles_terminate: forall c st
     (NOWHL: no_whiles c = true),
   exists st', c / st || st'.
 Proof.
-  exact FILL_IN_HERE.
+  intros. generalize dependent st.
+  induction c.
+  - intros. exists st. apply E_Skip.
+  - intros. exists (update st i (aeval st a)). apply E_Ass. reflexivity.
+  - intros.
+    assert (exists st' : state, c1 / st || st'). apply IHc1. simpl in NOWHL. rewrite andb_true_iff in NOWHL. apply NOWHL.
+    inversion H.
+    assert (exists st' : state, c2 / x || st'). apply IHc2. simpl in NOWHL. rewrite andb_true_iff in NOWHL. apply NOWHL.
+    inversion H1.
+    exists x0. apply E_Seq with x. apply H0. apply H2.
+  - intros.
+    assert (exists st' : state, c1 / st || st'). apply IHc1. simpl in NOWHL. rewrite andb_true_iff in NOWHL. apply NOWHL.
+    assert (exists st' : state, c2 / st || st'). apply IHc2. simpl in NOWHL. rewrite andb_true_iff in NOWHL. apply NOWHL.
+    remember (beval st b). destruct b0.
+    inversion H. exists x. apply E_IfTrue. symmetry. apply Heqb0. apply H1.
+    inversion H0. exists x. apply E_IfFalse. symmetry. apply Heqb0. apply H1.
+  - inversion NOWHL.
 Qed.
 
 (*-- Check --*)
